Preservation complete; working on progress

SporkProofs/Semantics.lean
@@ -136,7 +136,29 @@ end Expr
 inductive StackFrameCode : Type
   | code (c : Code)
   | cont (b : Cont)
-open StackFrameCode code cont
+-- open StackFrameCode code cont
+
+inductive SpawnCall : Type where
+  | mk (f : FuncIdx) (args : List Val) (ret : Nat)
+
+inductive SpawnDeque : Type where
+  -- unpromoted sporks, oldest first (queue)
+  -- promoted sporks, oldest last (stack)
+  | mk (unpr : List SpawnCall) (prom : SporkSig)
+
+inductive StackFrame : Type
+  | mk (f : FuncIdx)
+       (ρ : SpawnDeque)
+       (X : ValMap)
+       (c : StackFrameCode)
+
+inductive CallStack : Type where
+  | nil
+  | cons (K : CallStack) (k : StackFrame)
+
+inductive ThreadPool : Type where
+  | leaf : CallStack -> ThreadPool
+  | cat : ThreadPool -> ThreadPool -> ThreadPool
 
 namespace StackFrameCode
   -- instance instCoeToSum : Coe (Code ⊕ Cont) StackFrameCode where
@@ -193,9 +215,6 @@ namespace StackFrameCode
   deriving instance DecidableEq for StackFrameCode
 end StackFrameCode
 
-inductive SpawnCall : Type where
-  | mk (f : FuncIdx) (args : List Val) (ret : Nat)
-
 namespace SpawnCall
   abbrev f | mk f _args _ret => f
   abbrev args | mk _f args _ret => args
@@ -225,11 +244,6 @@ namespace SpawnCall
   deriving instance DecidableEq for SpawnCall
 end SpawnCall
 
-inductive SpawnDeque : Type where
-  -- unpromoted sporks, oldest first (queue)
-  -- promoted sporks, oldest last (stack)
-  | mk (unpr : List SpawnCall) (prom : SporkSig)
-
 namespace SpawnDeque
   abbrev unpr : SpawnDeque -> List SpawnCall
     | ⟨u, _p⟩ => u
@@ -238,9 +252,14 @@ namespace SpawnDeque
 
   abbrev SpawnOrder (canProm : Bool) (prom : SporkSig) : Prop :=
     prom = (if canProm then prom else [])
-  
-  theorem SpawnOrder_nil (canProm : Bool) : SpawnOrder canProm [] :=
-    by cases canProm <;> rfl
+
+  namespace SpawnOrder
+    theorem of_nil {canProm : Bool} : SpawnOrder canProm [] :=
+      by cases canProm <;> rfl
+    theorem prom_canProm_true : (canProm : Bool) -> {gret : Nat} -> {prom : SporkSig} ->
+                                SpawnOrder canProm (gret :: prom) -> canProm = true
+      | true, _gret, _prom, _so => rfl
+  end SpawnOrder
 
   inductive Okay (fsigs : FuncSigs) (canProm : Bool) : SpawnDeque -> Prop
     | mk {unpr : List SpawnCall} {prom : SporkSig} :
@@ -286,14 +305,8 @@ namespace SpawnDeque
   deriving instance DecidableEq for SpawnDeque
 
   theorem empty_okay {fsigs canProm} : SpawnDeque.Okay fsigs canProm ∅ :=
-    ⟨.nil, SpawnDeque.SpawnOrder_nil canProm⟩
+    ⟨.nil, .of_nil⟩
 end SpawnDeque
-
-inductive StackFrame : Type
-  | mk (f : FuncIdx)
-       (ρ : SpawnDeque)
-       (X : ValMap)
-       (c : StackFrameCode)
 
 namespace StackFrame
   abbrev f | mk f _ρ _X _c => f
@@ -373,10 +386,6 @@ namespace StackFrame
   deriving instance DecidableEq for StackFrame
 end StackFrame
 
-inductive CallStack : Type where
-  | nil
-  | cons (K : CallStack) (k : StackFrame)
-
 namespace CallStack
   notation (name := callstackcons) t " ⬝ " h:arg => cons t h
 
@@ -398,6 +407,8 @@ namespace CallStack
     | nil => []
     | K ⬝ k => unpr K ++ k.ρ.unpr
   abbrev allPromoted (K : CallStack) : Bool := K.unpr = []
+  abbrev allPromoted_imp_nil {K} (p : allPromoted K) : K.unpr = [] := by simp_all
+  abbrev nil_imp_allPromoted {K} (p : unpr K = []) : K.allPromoted := by simp_all
   abbrev firstFrame : (K : CallStack) -> K ≠ nil -> StackFrame
     | nil ⬝ k, p => k
     | K  ⬝ k ⬝ _k', p => firstFrame (K ⬝ k) (by simp)
@@ -483,16 +494,6 @@ namespace CallStack
                     ⟨Okay.cons kₒₖ, λ | Okay.cons _kₒₖ' Kₒₖ => Kₒₖ⟩)
         (isFalse ∘ λ | kₙₒₖ, .cons kₒₖ _Kₒₖ => kₙₒₖ kₒₖ)
 
-  -- instance instDecidableEq : DecidableEq CallStack
-  --   | nil, nil => isTrue rfl
-  --   | K ⬝ k, K' ⬝ k' =>
-  --     let KK'dec : Decidable (K = K') := instDecidableEq K K'
-  --     decidable_of_iff ((K = K') ∧ (k = k'))
-  --       ⟨λ ⟨Keq, keq⟩ => Keq ▸ keq ▸ rfl,
-  --        λ p => ⟨congrArg (λ | K ⬝ k => K | _ => K) p,
-  --                congrArg (λ | K ⬝ k => k | _ => k) p⟩⟩
-  --   | nil, K' ⬝ k' => isFalse (by simp)
-  --   | K' ⬝ k', nil => isFalse (by simp)
   deriving instance DecidableEq for CallStack
 
   abbrev retjoin?! {Pr get} : (K : CallStack) -> K.Okay Pr get -> Option Nat
@@ -546,11 +547,6 @@ namespace CallStack
   end Okay
 end CallStack
 
-
-inductive ThreadPool : Type where
-  | leaf : CallStack -> ThreadPool
-  | cat : ThreadPool -> ThreadPool -> ThreadPool
-
 namespace ThreadPool
   instance instAppend : Append ThreadPool where
     append := cat
@@ -574,8 +570,6 @@ namespace ThreadPool
     | cat {P P' ρ} :
           (Pₒₖ : P.Okay Pr (P'.retjoin Pr :: ρ)) ->
           (P'ₒₖ : P'.Okay Pr []) ->
-          -- P.prom.head? = some (P'.retjoin Pr) ->
-          -- P'.prom = [] ->
           (cat P P').Okay Pr ρ
 
   namespace Okay
@@ -585,13 +579,19 @@ namespace ThreadPool
       | cat _Pₒₖ P'ₒₖ => P'ₒₖ
     abbrev left {Pr P P' ρ} : (ok : (ThreadPool.cat P P').Okay Pr ρ) -> P.Okay Pr (P'.retjoin Pr :: ρ)
       | cat Pₒₖ _P'ₒₖ => Pₒₖ
+    
+    theorem same_prom {Pr} : {P : ThreadPool} -> {ρ : SporkSig} ->
+                      P.Okay Pr ρ -> P.prom = ρ
+      | .cat P₁ P₂, ρ, .cat P₁ₒₖ P₂ₒₖ =>
+        by simp[ThreadPool.prom, same_prom (ρ := P₂.retjoin Pr :: ρ) P₁ₒₖ]
+      | .leaf K, .(K.prom), .leaf Kₒₖ => rfl
   end Okay
 
   -- TODO: generalize for child threads not starting from main
-  abbrev init : ThreadPool := {{StackFrame.mk 0 ∅ ∅ (cont (Cont.mk 0 []))}}
+  abbrev init : ThreadPool := {{StackFrame.mk 0 ∅ ∅ (.cont (Cont.mk 0 []))}}
   abbrev child (f : FuncIdx) (args : List Val) : ThreadPool :=
     let vs := (List.range args.length).map Var.mk
-    {{StackFrame.mk f ∅ args (cont (Cont.mk 0 vs))}}
+    {{StackFrame.mk f ∅ args (.cont (Cont.mk 0 vs))}}
 
   instance instDecidable {Pr} : {ρ : SporkSig} -> (P : ThreadPool) -> Decidable (P.Okay Pr ρ)
     | ρ, leaf K => decidable_of_iff (ρ = K.prom ∧ K.Okay Pr none)
@@ -604,81 +604,96 @@ namespace ThreadPool
         ⟨λ ⟨Pₒₖ, P'ₒₖ⟩ => Okay.cat Pₒₖ P'ₒₖ,
          λ | Okay.cat Pₒₖ P'ₒₖ => ⟨Pₒₖ, P'ₒₖ⟩⟩
 
-  -- instance instDecidableEq : DecidableEq ThreadPool
-  --   | leaf K, leaf K' =>
-  --     decidable_of_iff (K = K')
-  --       ⟨congrArg leaf,
-  --        congrArg (λ | leaf K => K | _ => K)⟩
-  --   | cat Pₗ Pᵣ, cat Pₗ' Pᵣ' =>
-  --     match instDecidableEq Pₗ Pₗ', instDecidableEq Pᵣ Pᵣ' with
-  --       | isFalse f, _ => isFalse (f ∘ congrArg (λ | cat l r => l | _ => Pₗ))
-  --       | _, isFalse f => isFalse (f ∘ congrArg (λ | cat l r => r | _ => Pᵣ))
-  --       | isTrue tₗ, isTrue tᵣ => isTrue (tₗ ▸ tᵣ ▸ rfl)
-  --   | leaf _, cat _ _ => isFalse (by simp)
-  --   | cat _ _, leaf _ => isFalse (by simp)
   deriving instance DecidableEq for ThreadPool
 
-  -- abbrev step (Pr : Program) : ThreadPool -> Option ThreadPool
-  --   | leaf (K ⬝ ⟨f, ρ, X, code (.stmt e c)⟩) =>
-  --     if ok : e.Okay X.length then
-  --       some {K ⬝ e.eval X ok}
+
+  inductive Okay' (Pr : Program) : ThreadPool -> Prop where
+    | leaf {K} :
+           (Kₒₖ : K.Okay Pr none) ->
+           (leaf K).Okay' Pr
+    | cat {P P'} :
+          (Pₒₖ : P.Okay' Pr) ->
+          (P'ₒₖ : P'.Okay' Pr) ->
+          (P.prom.head? = some (P'.retjoin Pr)) ->
+          (P'.prom = []) ->
+          (cat P P').Okay' Pr
+
+  namespace Okay
+    theorem to_okay' {Pr : Program} : {P : ThreadPool} -> {ρ : SporkSig} ->
+                     P.Okay Pr ρ -> P.Okay' Pr
+      | .leaf K, .(K.prom), .leaf Kₒₖ =>
+        .leaf Kₒₖ
+      | .cat _P _P', _ρ, .cat Pₒₖ P'ₒₖ =>
+        .cat Pₒₖ.to_okay' P'ₒₖ.to_okay'
+          (Pₒₖ.same_prom ▸ rfl) P'ₒₖ.same_prom
+  end Okay
+
+  namespace Okay'
+    theorem to_okay {Pr : Program} : {P : ThreadPool} ->
+                     P.Okay' Pr -> P.Okay Pr P.prom
+      | .leaf K, .leaf Kₒₖ =>
+        .leaf Kₒₖ
+      | .cat P P', .cat Pₒₖ P'ₒₖ Pprom P'prom =>
+        match x : P.prom with
+          | Ppromh :: Ppromt =>
+            let x'' : Ppromh = retjoin Pr P' :=
+              congrArg (λ | some h => h | none => Ppromh) (x ▸ Pprom)
+            by simp![x]
+               exact .cat (ρ := Ppromt) (x'' ▸ x ▸ Pₒₖ.to_okay) (P'prom ▸ P'ₒₖ.to_okay)
+          | [] => let y := x ▸ Pprom
+                  by contradiction
+  end Okay'
+
+  theorem okay_iff_okay' {Pr : Program} {P : ThreadPool} : P.Okay Pr P.prom <-> P.Okay' Pr :=
+    ⟨Okay.to_okay', Okay'.to_okay⟩
 
 end ThreadPool
 
 
 @[inline] abbrev codeOf (Pr : Program) (f : FuncIdx) (b : Cont) : StackFrameCode :=
-  code Pr.funs[f]!.blocks[b.b]!.code
+  .code Pr.funs[f]!.blocks[b.b]!.code
 @[inline] abbrev codeEntry (Pr : Program) (f : FuncIdx) : StackFrameCode :=
-  code Pr.funs[f]!.blocks.head!.code
-
-theorem codeOfGetElem {Pr : Program} {f : FuncIdx} {b : Cont}
-                    (pf : f < Pr.size) (pb : b.b < Pr.funs[f].blocks.length) :
-                    Pr.funs[f]!.blocks[b.b]! = Pr.funs[f].blocks[b.b] :=
-  by rw[getElem!_pos Pr.funs f pf, getElem!_pos Pr.funs[f].blocks b.b pb]
-
-theorem argsOfGetElem {x : List Var} {X : ValMap} (ok : IVec (·.Okay X.length) x):
-                    X[x]! = X[x] :=
-  getElem!_pos X x ok
+  .code Pr.funs[f]!.blocks.head!.code
 
 inductive Step (Pr : Program) : (P P' : ThreadPool) -> Type where
   | stepₗ {P P' P₂} :
     Step Pr P P' ->
-    Step Pr (P ++ P₂) (P' ++ P₂)
+    Step Pr (.cat P P₂) (.cat P' P₂)
 
   | stepᵣ {P₁ P P'} :
     Step Pr P P' ->
-    Step Pr (P₁ ++ P) (P₁ ++ P')
+    Step Pr (.cat P₁ P) (.cat P₁ P')
   
   | stmt {f K ρ X e v c} :
     X ⊢ₑₓₚᵣ e ⇓ v ->
-    Step Pr {K ⬝ ⟨f, ρ, X, code (Code.stmt e c)⟩}
-            {K ⬝ ⟨f, ρ, X ++ [v], code c⟩}
+    Step Pr {K ⬝ ⟨f, ρ, X, .code (.stmt e c)⟩}
+            {K ⬝ ⟨f, ρ, X ++ [v], .code c⟩}
 
   | goto {f K ρ X bnext} :
-    Step Pr {K ⬝ ⟨f, ρ, X, code (Code.trfr (Transfer.goto bnext))⟩}
+    Step Pr {K ⬝ ⟨f, ρ, X, .code (.trfr (.goto bnext))⟩}
             {K ⬝ ⟨f, ρ, X[bnext.args]!, codeOf Pr f bnext⟩}
 
   | ite_true {f K ρ X cond bthen belse n} :
     X ⊢ₐₜₒₘ cond ⇓ n ->
     n ≠ 0 ->
-    Step Pr {K ⬝ ⟨f, ρ, X, code (Code.trfr (Transfer.ite cond bthen belse))⟩}
+    Step Pr {K ⬝ ⟨f, ρ, X, .code (.trfr (.ite cond bthen belse))⟩}
             {K ⬝ ⟨f, ρ, X[bthen.args]!, codeOf Pr f bthen⟩}
 
   | ite_false {f K ρ X cond bthen belse} :
     X ⊢ₐₜₒₘ cond ⇓ 0 ->
-    Step Pr {K ⬝ ⟨f, ρ, X, code (Code.trfr (Transfer.ite cond bthen belse))⟩}
+    Step Pr {K ⬝ ⟨f, ρ, X, .code (.trfr (.ite cond bthen belse))⟩}
             {K ⬝ ⟨f, ρ, X[belse.args]!, codeOf Pr f belse⟩}
 
   | call {f g K ρ X x bret} :
-    Step Pr {K ⬝ ⟨f, ρ, X, code (Code.trfr (Transfer.call g x bret))⟩}
-            {K ⬝ ⟨f, ρ, X, cont bret⟩ ⬝ ⟨g, {}, X[x]!, codeEntry Pr g⟩}
+    Step Pr {K ⬝ ⟨f, ρ, X, .code (.trfr (.call g x bret))⟩}
+            {K ⬝ ⟨f, ρ, X, .cont bret⟩ ⬝ ⟨g, {}, X[x]!, codeEntry Pr g⟩}
 
   | retn {f g K ρ X Y y bret} :
-    Step Pr {K ⬝ ⟨f, ρ, X, cont bret⟩ ⬝ ⟨g, {}, Y, code (Code.trfr (Transfer.retn y))⟩}
+    Step Pr {K ⬝ ⟨f, ρ, X, .cont bret⟩ ⬝ ⟨g, {}, Y, .code (.trfr (.retn y))⟩}
             {K ⬝ ⟨f, ρ, X[bret.args]! ++ Y[y]!, codeOf Pr f bret⟩}
 
   | spork {f K ρ X g g_args bbody} :
-    Step Pr {K ⬝ ⟨f, ρ, X, code (Code.trfr (Transfer.spork bbody g g_args))⟩}
+    Step Pr {K ⬝ ⟨f, ρ, X, .code (.trfr (.spork bbody g g_args))⟩}
             {K ⬝ ⟨f, ρ.push ⟨g, X[g_args]!, Pr.funs[g]!.fsig.ret⟩, X[bbody.args]!, codeOf Pr f bbody⟩}
 
   | promote {f unpr g prom X K c K'} :
@@ -689,315 +704,22 @@ inductive Step (Pr : Program) : (P P' : ThreadPool) -> Type where
              {⟨g.f, {}, g.args, codeEntry Pr g.f⟩}}
 
   | spoin_unpr {f K ρ sc X bunpr bprom} :
-    Step Pr {K ⬝ ⟨f, ρ.push sc, X, code (Code.trfr (Transfer.spoin bunpr bprom))⟩}
+    Step Pr {K ⬝ ⟨f, ρ.push sc, X, .code (.trfr (.spoin bunpr bprom))⟩}
             {K ⬝ ⟨f, ρ, X[bunpr.args]!, codeOf Pr f bunpr⟩}
 
   | spoin_prom {f K ρ X bunpr bprom Y y} {g : SpawnCall} :
     K.unpr = [] ->
-    Step Pr {(K ⬝ ⟨f, ⟨[], g.ret :: ρ⟩, X, code (Code.trfr (Transfer.spoin bunpr bprom))⟩),
-             {⟨g.f, {}, Y, code (Code.trfr (Transfer.retn y))⟩}}
+    Step Pr {(K ⬝ ⟨f, ⟨[], g.ret :: ρ⟩, X, .code (.trfr (.spoin bunpr bprom))⟩),
+             {⟨g.f, {}, Y, .code (.trfr (.retn y))⟩}}
             {K ⬝ ⟨f, ⟨[], ρ⟩, X[bprom.args]! ++ Y[y]!, codeOf Pr f bprom⟩}
-
-namespace Step
-  notation (name := poolstep) Pr:arg " ⊢ " P:arg " ↦ " P':arg => Step Pr P P'
-
-  theorem preserve_retjoin_stack_cons
-    {Pr K f ρ ρ' X X' c c'} :
-      CallStack.retjoin Pr (K ⬝ ⟨f, ρ, X, c⟩) =
-        CallStack.retjoin Pr (K ⬝ ⟨f, ρ', X', c'⟩)
-    := by cases K <;> rfl
-
-  theorem preserve_retjoin_stack_cons_cons {Pr K k k'} :
-      (K ⬝ k ⬝ k').retjoin Pr = (K ⬝ k).retjoin Pr :=
-    by cases K <;> rfl
-
-  theorem preserve_retjoin_stack_cons_nonnil {Pr K k} :
-      K ≠ ∅ → (K ⬝ k).retjoin Pr = K.retjoin Pr := by
-    cases K <;> intro nn
-    · case nil => contradiction
-    · case cons => rfl
-
-  -- List.append_ne_nil_of_left_ne_nil
-  theorem stack_append_left_nonnil : (s t : CallStack) -> (h : s ≠ ∅) -> s ++ t ≠ ∅
-    | s, .nil, h => h
-    | s, K ⬝ k, h => by simp
-
-  theorem preserve_retjoin_stack_append {Pr K k} : {K' : CallStack} ->
-      CallStack.retjoin Pr (K ⬝ k ++ K') = CallStack.retjoin Pr (K ⬝ k)
-    | .nil => rfl
-    | K' ⬝ k' => preserve_retjoin_stack_cons_nonnil
-                   (stack_append_left_nonnil (K ⬝ k) K' (by simp)) ▸
-                 preserve_retjoin_stack_append (K' := K')
-
-  theorem preserve_retjoin {Pr : Program} : {P P' : ThreadPool} ->
-                         Pr ⊢ P ↦ P' -> {ρ : SporkSig} -> P.Okay Pr ρ ->
-                         P.retjoin Pr = P'.retjoin Pr
-  | P, P', s => by
-    cases s <;> intro Pₒₖ <;>
-    try (exact preserve_retjoin_stack_cons)
-    · case stepₗ P P' P₂ s =>
-        simp_all!; match Pₒₖ with
-          | .cat Pok P2ok => exact preserve_retjoin s Pok
-    · case stepᵣ P₁ P P' s =>
-        rfl
-    · case retn f g K ρ' X Y y bret =>
-        exact preserve_retjoin_stack_cons (K := K)
-    · case promote f unpr g prom X K c K' u p =>
-        simp[ThreadPool.retjoin];
-        rw[preserve_retjoin_stack_append,
-           preserve_retjoin_stack_append,
-           preserve_retjoin_stack_cons]
-
-  theorem goto_okay_rets
-      {Pr} (Prok : Pr.Okay) {f canProm ρ} {X Y : ValMap} {bnext} {y : List Var}
-      (p : f < Pr.size)
-      (ρok : ρ.Okay Pr.fsigs canProm)
-      (bnext_ok : bnext.OkayRets Pr.funs[f].bsigs ⟨X.length, ρ.sig⟩ y.length)
-      (y_ok : IVec (·.Okay Y.length) y) :
-      StackFrame.Okay Pr none canProm
-        ⟨f, ρ, X[bnext.args]! ++ Y[y]!, codeOf Pr f bnext⟩ :=
-    let ⟨bok, sigok, x_ok⟩ := bnext_ok
-    let bok' : bnext.b < Pr.funs[f].blocks.length :=
-      List.length_map Block.bsig ▸ bok
-    let xlen : bnext.args.length = X[bnext.args].length :=
-      x_ok.map_length (λ x xₒₖ => X[x])
-    let ylen : y.length = Y[y].length :=
-      y_ok.map_length (λ y yₒₖ => Y[y])
-    let code_ok : Pr.funs[f]!.blocks[bnext.b]!.code.Okay
-                    Pr.fsigs Pr.funs[f].bsigs Pr.funs[f].fsig.ret
-                    ⟨(X[bnext.args]! ++ Y[y]!).length, ρ.sig⟩ := by
-      rw[codeOfGetElem p bok',
-         argsOfGetElem x_ok,
-         argsOfGetElem y_ok,
-         List.length_append,
-         ← xlen, ← ylen, ← sigok]
-      simp; exact ((Prok.1.get ⟨f, p⟩).1.get ⟨bnext.b, bok'⟩).1
-    ⟨p, ρok, rfl, .code code_ok⟩
-
-  theorem goto_okay
-      {Pr} (Prok : Pr.Okay) {f canProm ρ} {X : ValMap} {bnext}
-      (p : f < Pr.size)
-      (ρok : ρ.Okay Pr.fsigs canProm)
-      (bnext_ok : bnext.Okay Pr.funs[f].bsigs ⟨X.length, ρ.sig⟩) :
-      StackFrame.Okay Pr none canProm ⟨f, ρ, X[bnext.args]!, codeOf Pr f bnext⟩ :=
-    List.append_nil X[bnext.args]! ▸
-    goto_okay_rets Prok (Y := []) (y := []) p ρok bnext_ok.cast0 .nil
-
-  theorem entry_okay
-      {Pr} (Prok : Pr.Okay) {f canProm} {X : List Val}
-      (p : f < Pr.size)
-      (sigok : Pr.funs[f].fsig.arity = X.length) :
-      StackFrame.Okay Pr none canProm ⟨f, ∅, X, codeEntry Pr f⟩ :=
-    let fok := Prok.1.get ⟨f, p⟩
-    let c' : Code.Okay Pr.fsigs Pr.funs[f].bsigs Pr.funs[f].fsig.ret
-              ⟨X.length, []⟩
-              Pr.funs[f]!.blocks.head!.code :=
-      sigok ▸
-      Eq.symm (getElem!_pos Pr.funs f p) ▸
-      fok.2.headeq ▸
-      fok.2.head!eq ▸
-      (fok.1.head fok.2.nonnil).1
-    ⟨p, SpawnDeque.empty_okay, rfl, .code c'⟩
-
-  theorem goto_entry_okay
-      {Pr} (Prok : Pr.Okay) {f canProm} {X : ValMap} {x : List Var}
-      (p : f < Pr.size)
-      (xok : IVec (·.Okay X.length) x)
-      (sigok : Pr.funs[f].fsig.arity = x.length) :
-      StackFrame.Okay Pr none canProm ⟨f, ∅, X[x]!, codeEntry Pr f⟩ :=
-    entry_okay Prok p (argsOfGetElem xok ▸
-                       xok.map_length (λ x xₒₖ => X[x]) ▸
-                       sigok)
-
-  theorem P_same_prom {Pr} : {P : ThreadPool} -> {ρ : SporkSig} ->
-                    P.Okay Pr ρ -> P.prom = ρ
-    | .cat P₁ P₂, ρ, .cat P₁ₒₖ P₂ₒₖ =>
-      by simp[ThreadPool.prom]
-         rw[P_same_prom (ρ := P₂.retjoin Pr :: ρ) P₁ₒₖ]
-         simp
-    | .leaf K, .(K.prom), .leaf Kₒₖ =>
-      rfl
-
-  theorem leaf' {Pr} {K : CallStack} (ρ : SporkSig) (p : ρ = K.prom) (Kₒₖ : K.Okay Pr none) : (ThreadPool.leaf K).Okay Pr ρ :=
-    p ▸ .leaf Kₒₖ
-  
-  open ThreadPool.Okay (leaf cat) in
-  theorem preservation {Pr : Program} (Prok : Pr.Okay) : {P P' : ThreadPool} -> {ρ : SporkSig} -> P.Okay Pr ρ -> Pr ⊢ P ↦ P' -> P'.Okay Pr ρ := by
-    intro P P' ρ ok P_P'; cases P_P' <;> cases ok
-
-    · case stepₗ P P' P₂ P_P' P2ok Pok =>
-        exact cat (preservation Prok Pok P_P') P2ok
-
-    · case stepᵣ P₁ P P' P_P' Pok P1ok =>
-        exact cat (preserve_retjoin P_P' Pok ▸ P1ok) (preservation Prok Pok P_P')
-
-    · case stmt f K ρ X e v c a ok =>
-        apply @leaf Pr (K ⬝ ⟨f, ρ, X ++ [v], code c⟩)
-        exact match ok with
-           | Kok ⬝ₒₖ (.mk p ρok _ (.code (.stmt eok cok))) =>
-             Kok ⬝ₒₖ (.mk p ρok rfl (.code
-                 (by simp[BlockSig.bind] at cok; simp; exact cok)))
-
-    · case goto f K ρ X bnext ok =>
-        apply @leaf Pr (K ⬝ ⟨f, ρ, X[bnext.args]!, codeOf Pr f bnext⟩)
-        exact match ok with
-          | Kok ⬝ₒₖ (.mk p ρok _ (.code (.trfr (.goto bnext_ok))))=>
-            Kok ⬝ₒₖ (goto_okay Prok p ρok bnext_ok)
-
-    · case ite_true f K ρ X cond bthen belse n cond_n neq0 ok =>
-        apply @leaf Pr (K ⬝ ⟨f, ρ, X[bthen.args]!, codeOf Pr f bthen⟩)
-        exact match ok with
-          | Kok ⬝ₒₖ (.mk p ρok _ (.code (.trfr (.ite cond_ok bthen_ok belse_ok)))) =>
-            Kok ⬝ₒₖ (goto_okay Prok p ρok bthen_ok)
-
-    · case ite_false f K ρ X cond bthen belse cond_0 ok =>
-        apply @leaf Pr (K ⬝ ⟨f, ρ, X[belse.args]!, codeOf Pr f belse⟩)
-        exact match ok with
-          | Kok ⬝ₒₖ (.mk p ρok _ (.code (.trfr (.ite cond_ok bthen_ok belse_ok)))) =>
-            Kok ⬝ₒₖ (goto_okay Prok p ρok belse_ok)
-
-    · case call f g K ρ X x bret ok =>
-        apply @leaf Pr (K ⬝ ⟨f, ρ, X, cont bret⟩ ⬝ ⟨g, ∅, X[x]!, codeEntry Pr g⟩)
-        exact match ok with
-          | Kok ⬝ₒₖ kok@(.mk fok ρok _ (.code (.trfr (.call flt sigok x_ok
-                bret_ok@(.mk bret_lt bret_sig_okay argsok))))) =>
-              let bret_ok' : Cont.OkayRets Pr.funs[f].bsigs ⟨X.length, ρ.sig⟩
-                               Pr.fsigs[g].ret bret :=
-                Pr.funs.getElem_map (·.fsig) ▸ bret_ok
-              let gframe_ok :=
-                goto_entry_okay (f := g) Prok (Pr.size_eq_fsigs_length ▸ flt) x_ok
-                  (Pr.funs.getElem_map (·.fsig) ▸ sigok)
-              let glt := gframe_ok.flt
-              let bret_ok'' : Cont.OkayRets Pr.funs[f].bsigs ⟨X.length, ρ.sig⟩
-                                Pr.funs[g].fsig.ret bret :=
-                Pr.funs.getElem_map (·.fsig) ▸ bret_ok'
-              Kok ⬝ₒₖ ⟨fok, ρok, rfl, .cont bret_ok''⟩ ⬝ₒₖ gframe_ok
-
-    · case retn f g K ρ X Y y bret ok =>
-        apply @leaf Pr (K ⬝ ⟨f, ρ, X[bret.args]! ++ Y[y]!, codeOf Pr f bret⟩)
-        exact match ok with
-          | Kok ⬝ₒₖ (.mk flt ρok _ (.cont bret_ok))
-                ⬝ₒₖ (.mk glt ⟨.nil, _⟩ _ (.code (.trfr (.retn _ ylen y_ok)))) =>
-            Kok ⬝ₒₖ (goto_okay_rets Prok flt ρok (ylen ▸ bret_ok) y_ok)
-
-    · case spork f K ρ X g g_args bbody ok =>
-       apply @leaf Pr (K ⬝ ⟨f, ρ.push ⟨g, X[g_args]!, Pr.funs[g]!.fsig.ret⟩,
-                            X[bbody.args]!, codeOf Pr f bbody⟩)
-       exact match ok with
-         | Kok ⬝ₒₖ ⟨flt, ⟨unpr_ok, prom_ok⟩, _, .code
-               (.trfr (.spork glt gsig g_args_ok bbody_ok))⟩ =>
-           let glt' : g < Pr.funs.length := List.length_map (α := Func) (·.fsig) ▸ glt
-           let h : FuncSig.mk X[g_args]!.length Pr.funs[g]!.fsig.ret = Pr.fsigs[g] :=
-             argsOfGetElem g_args_ok ▸
-             getElem!_pos Pr.funs g glt' ▸
-             congrArg₂ FuncSig.mk
-               (g_args_ok.map_length (λ x xₒₖ => X[x]) ▸ Eq.symm gsig) (by simp)
-           Kok ⬝ₒₖ (goto_okay Prok flt ⟨unpr_ok.append (IVec.singleton ⟨glt, h⟩), prom_ok⟩
-                     (by rw[ρ.pushsig, getElem!_pos Pr.funs g glt']
-                         simp[BlockSig.spork] at bbody_ok; simp
-                         exact bbody_ok))
-
-    · case promote f unpr g prom X K c K' u p ok =>
-        let kProm : K.allPromoted = true := by simp_all
-        let rec hp : {K' : CallStack} -> {gets : Option Nat} -> K'.prom = [] ->
-                     CallStack.Okay Pr gets (K ⬝ ⟨f, ⟨g :: unpr, prom⟩, X, c⟩ ++ K') ->
-                     CallStack.Okay Pr gets (K ⬝ ⟨f, ⟨unpr, g.ret :: prom⟩, X, c⟩ ++ K') ∧
-                     CallStack.Okay Pr none {⟨g.f, ∅, g.args, codeEntry Pr g.f⟩} ∧
-                     g.ret = Pr.funs[g.f]!.fsig.ret
-          | .nil, gets, _, ok => by
-            rw[CallStack.append_nil] at *
-            apply And.intro <;> try (apply And.intro)
-            · exact ok.tail ⬝ₒₖ
-                (let kok := ok.head
-                 ⟨ok.head.flt,
-                  (let x := ok.head.ρₒₖ
-                   by rw[kProm] at *
-                      exact x.promote),
-                  ok.head.cb,
-                  ok.head.cₒₖ
-                  ⟩)
-            · apply (.nil ⬝ₒₖ ·)
-              let glt : g.f < Pr.funs.length := by
-                rw[← List.length_map (·.fsig)]
-                exact ok.head.ρₒₖ.unpr.head'.flt
-              let Prsize : Pr.funs.length = Pr.fsigs.length :=
-                (List.length_map (as := Pr.funs) (·.fsig)).symm
-              let glt' := Prsize ▸ glt
-              exact StackFrame.Okay.mk glt SpawnDeque.empty_okay rfl
-                (entry_okay (canProm := true) Prok glt
-                  (List.getElem_map Func.fsig (l := Pr.funs) ▸
-                   (congrArg (·.arity) ok.head.ρₒₖ.unpr.head'.sig).symm)
-                ).cₒₖ
-            · let gflt := ok.head.ρₒₖ.unpr.head'.flt
-              let gflt' : g.f < Pr.funs.length :=
-                List.length_map (as := Pr.funs) (·.fsig) ▸ gflt
-              let x : g.ret = Pr.fsigs[g.f].ret :=
-                congrArg (·.ret) ok.head.ρₒₖ.unpr.head'.sig
-              rw[getElem!_pos Pr.funs g.f gflt',
-                 x,
-                 List.getElem_map (·.fsig) (l := Pr.funs)]
-          | K' ⬝ k', gets, p, ok =>
-            let ⟨kp', Kp'⟩ := List.append_eq_nil_iff.mp p
-            let k'ok := ok.head
-            let ⟨K'ok', gok, glt⟩ := hp Kp' ok.tail
-            let l := K'ok'
-            let k'ok' := k'ok.castCanProm
-              (K ⬝ ⟨f, ⟨unpr, g.ret :: prom⟩, X, c⟩ ++ K').allPromoted
-              (λ (x : (K ⬝ ⟨f, ⟨g :: unpr, prom⟩, X, c⟩ ++ K').allPromoted) =>
-                 let x' : (K ⬝ ⟨f, ⟨g :: unpr, prom⟩, X, c⟩ ++ K').unpr = [] :=
-                   by simp_all[x]
-                 let x'' : g :: unpr = [] :=
-                   (List.append_eq_nil_iff.mp
-                     (List.append_eq_nil_iff.mp
-                       (CallStack.append_unpr ▸ x')).left).right
-                 by contradiction)
-            ⟨K'ok' ⬝ₒₖ k'ok', gok, glt⟩
-        let ⟨Kok, gok, glt⟩ := hp p ok
-        let prom_p : Pr.funs[g.f]!.fsig.ret ::
-                       (K ⬝ ⟨f, ⟨g :: unpr, prom⟩, X, c⟩ ++ K').prom =
-                     (K ⬝ ⟨f, ⟨unpr, g.ret :: prom⟩, X, c⟩ ++ K').prom := by
-          simp_all[CallStack.append_prom, p, glt]
-        exact cat (prom_p ▸ leaf Kok) (leaf gok)
-
-    · case spoin_unpr f K ρ sc X bunpr bprom ok =>
-        apply @leaf Pr (K ⬝ ⟨f, ρ, X[bunpr.args]!, codeOf Pr f bunpr⟩)
-        exact match ok with
-          | Kok ⬝ₒₖ ⟨flt, ⟨unpr_ok, prom_ok⟩, _,
-              .code (.trfr (.spoin nn bunpr_ok bprom_ok))⟩ =>
-            let h : (ρ.push sc).sig.tail = ρ.sig := by simp
-            Kok ⬝ₒₖ (goto_okay Prok flt ⟨unpr_ok.unappend.1, prom_ok⟩ (h ▸ bunpr_ok))
-
-    · case spoin_prom f K ρ' X bunpr bprom Y y g K_unpr_nil retok ok =>
-        let p : g.ret :: ρ' ++ K.prom = Pr.funs[g.f]!.fsig.ret :: ρ :=
-          P_same_prom ok
-        let g_ret_eq : g.ret = Pr.funs[g.f]!.fsig.ret :=
-          congrArg (λ | some x => x | _ => g.ret) (congrArg List.head? p)
-        let ρ_eq_ρ'_Kprom : ρ = ρ' ++ K.prom :=
-          Eq.symm (congrArg List.tail p)
-        rw[ρ_eq_ρ'_Kprom] at ok ⊢
-        apply @leaf Pr (K ⬝ ⟨f, ⟨[], ρ'⟩, X[bprom.args]! ++ Y[y]!, codeOf Pr f bprom⟩)
-        let ok'' : (ThreadPool.leaf (K ⬝ ⟨f, ⟨[], g.ret :: ρ'⟩, X,
-                      code (.trfr (.spoin bunpr bprom))⟩)).Okay Pr (g.ret :: ρ' ++ K.prom) :=
-          g_ret_eq ▸ ok
-        let flt := ok''.get.head.flt
-        let sd_ok : (SpawnDeque.mk [] ρ').Okay Pr.fsigs K.allPromoted :=
-          ⟨IVec.nil, by simp[CallStack.allPromoted]; rw[K_unpr_nil]; rfl⟩
-        let y_ok : IVec (·.Okay Y.length) y :=
-          match retok.get.head.cₒₖ.c.t with
-            | .retn _ _ y_ok => y_ok
-        let y_len_eq_g_ret : y.length = g.ret :=
-          match retok.get.head.cₒₖ'.c.t with
-            | .retn _ l _ => g_ret_eq ▸ Eq.symm l
-        let cont_ok : bprom.OkayRets Pr.funs[f].bsigs ⟨X.length, ρ'⟩ y.length :=
-          match ok''.get.head.cₒₖ.c.t with
-            | .spoin nn unpr_ok prom_ok => y_len_eq_g_ret ▸ prom_ok
-        exact ok''.get.tail ⬝ₒₖ
-          (goto_okay_rets Prok flt sd_ok cont_ok y_ok)
-end Step
 
 inductive Steps (Pr : Program) : (P P' : ThreadPool) -> Type where
   | nil {P : ThreadPool} : Steps Pr P P
-  | cons {P P' P'' : ThreadPool} : Steps Pr P P' -> Pr ⊢ P' ↦ P'' -> Steps Pr P P''
+  | cons {P P' P'' : ThreadPool} : Steps Pr P P' -> Step Pr P' P'' -> Steps Pr P P''
+
+namespace Step
+  notation (name := poolstep) Pr:arg " ⊢ " P:arg " ↦ " P':arg => Step Pr P P'
+end Step
 
 namespace Steps
   notation (name := stepsstep) Pr:arg " ⊢ " P:arg " ↦* " P':arg => Steps Pr P P'
@@ -1007,8 +729,17 @@ namespace Steps
     | _P, _P', .(_P'), ss', nil => ss'
     | _P, _P', _P'', ss', cons ss s => cons (append ss' ss) s
   instance instHAppend {Pr : Program} {P P' P'' : ThreadPool} :
-                       HAppend (Pr ⊢ P ↦* P') (Pr ⊢ P' ↦* P'') (Pr ⊢ P ↦* P'') :=
-    ⟨append⟩
-  instance instSingleton {Pr : Program} {P P' : ThreadPool} : Singleton (Pr ⊢ P ↦ P') (Pr ⊢ P ↦* P') :=
-    ⟨λ s => cons nil s⟩
+                       HAppend (Pr ⊢ P ↦* P') (Pr ⊢ P' ↦* P'') (Pr ⊢ P ↦* P'') where
+    hAppend := append
+  instance instSingleton {Pr : Program} {P P' : ThreadPool} : Singleton (Pr ⊢ P ↦ P') (Pr ⊢ P ↦* P') where
+    singleton := cons nil
 end Steps
+
+theorem codeOfGetElem {Pr : Program} {f : FuncIdx} {b : Cont}
+                    (pf : f < Pr.size) (pb : b.b < Pr.funs[f].blocks.length) :
+                    Pr.funs[f]!.blocks[b.b]! = Pr.funs[f].blocks[b.b] :=
+  by rw[getElem!_pos Pr.funs f pf, getElem!_pos Pr.funs[f].blocks b.b pb]
+
+theorem argsOfGetElem {x : List Var} {X : ValMap} (ok : IVec (·.Okay X.length) x):
+                    X[x]! = X[x] :=
+  getElem!_pos X x ok
