SporkProofs/Progress.lean
@@ -1,0 +1,78 @@
+import SporkProofs.Syntax
+import SporkProofs.Semantics
+import SporkProofs.Preservation
+
+namespace Step
+
+  inductive Next (Pr : Program) : ThreadPool -> Type where
+    | result (g X x) :
+        Next Pr {{⟨g, ∅, X, .code (.trfr (.retn x))⟩}}
+    | blocked (K f gret ρ X bunpr bprom) :
+        Next Pr {K ⬝ ⟨f, ⟨[], gret :: ρ⟩, X, .code (.trfr (.spoin bunpr bprom))⟩}
+    | step {P} (P') (s : Pr ⊢ P ↦ P') :
+        Next Pr P
+
+  theorem prom_imp_allPromoted
+      {Pr K get f gret ρ X c}
+      (ok : (K ⬝ ⟨f, ⟨[], gret :: ρ⟩, X, c⟩).Okay Pr get) :
+      K.unpr = [] :=
+    K.allPromoted_imp_nil
+      (ok.head.ρₒₖ.prom.prom_canProm_true K.allPromoted)
+  
+  def progress {Pr : Program} : -- (Prok : Pr.Okay) :
+               (P : ThreadPool) -> P.Okay' Pr ->
+               Next Pr P
+    | .cat P₁ P₂, ok =>
+      let P₁ok : P₁.Okay' Pr := ok.to_okay.left.to_okay'
+      let P₂ok := ok.to_okay.right.to_okay'
+      match progress P₁ P₁ok with
+        | .result g X x =>
+          let y := ok.to_okay.left.same_prom;
+          by contradiction
+        | .step P₁' s =>
+          .step _ (.stepₗ s)
+        | .blocked K f gret ρ X bunpr bprom =>
+          let P₁b : ThreadPool :=
+            {K ⬝ ⟨f, ⟨[], gret :: ρ⟩, X, .code (.trfr (.spoin bunpr bprom))⟩}
+          let P₁bok : P₁b.Okay' Pr := ok.to_okay.left.to_okay'
+          match progress P₂ P₂ok with
+            | .result g Y y =>
+              .step _ (.spoin_prom (g := ⟨g, default /- doesn't matter -/, gret⟩)
+                         (prom_imp_allPromoted ok.to_okay.left.get))
+            | .blocked K' f' gret' ρ' X' bunpr' bprom' =>
+              let z := ok.to_okay.right.same_prom
+              by contradiction
+            | .step P₂' s =>
+              .step _ (.stepᵣ s)
+    | .leaf (K ⬝ ⟨f, ρ, X, .code (.stmt e c)⟩), ok =>
+      let eₒₖ := ok.to_okay.get.head.cₒₖ.c.e
+      .step _ (.stmt (Expr.Eval.mk eₒₖ))
+    | .leaf (K ⬝ ⟨f, ρ, X, .code (.trfr (.goto bnext))⟩), ok =>
+      .step _ .goto
+    | .leaf (K ⬝ ⟨f, ρ, X, .code (.trfr (.ite cond bthen belse))⟩), ok =>
+      let condₒₖ := match ok.to_okay.get.head.cₒₖ.c.t with
+        | .ite condₒₖ bthenₒₖ belseₒₖ => condₒₖ
+      let c? := cond.eval X condₒₖ
+      if p : c? = 0 then
+        .step _ (.ite_false (p ▸ .mk condₒₖ))
+      else
+        .step _ (.ite_true (.mk condₒₖ) p)
+    | .leaf (K ⬝ ⟨f, ρ, X, .code (.trfr (.call g args bret))⟩), ok =>
+      .step _ .call
+    | .leaf (K ⬝ ⟨f, ρ, X, .cont bnext⟩ ⬝ ⟨g, ρempty, Y, .code (.trfr (.retn y))⟩), ok =>
+      let p : ρempty = ∅ :=
+        by cases ρempty; cases ok.to_okay.get.head.cₒₖ.c.t; simp_all; rfl
+      p ▸ .step _ .retn
+    | .leaf (K ⬝ ⟨f, ρ, X, .code c⟩ ⬝ ⟨g, ρempty, Y, .code (.trfr (.retn y))⟩), ok =>
+      let x := ok.to_okay.get.tail.head.isCont
+      by contradiction
+    | .leaf (.nil ⬝ ⟨g, ρempty, Y, .code (.trfr (.retn y))⟩), ok =>
+      let p : ρempty = ∅ :=
+        by cases ρempty; cases ok.to_okay.get.head.cₒₖ.c.t; simp_all; rfl
+      p ▸ .result g Y y
+    | .leaf (K ⬝ ⟨f, ρ, X, .code (.trfr (.spork bbody g args))⟩), ok =>
+      sorry
+    | .leaf (K ⬝ ⟨f, ρ, X, .code (.trfr (.spoin bunpr bprom))⟩), ok =>
+      -- either spoin_unpr or spoin_prom->blocked
+      sorry
+end Step
